simple ffi examples
simple ffi examples

- store effect is now more general (can be polymorphic in ctx dep bit)
- delimlang embedded into a language with higher-order heap
- type system + interpretation + safety wrt GITree eq. th.
- an example without glue code, which is well-typed, but
  unguarded shift captures heap lang ctx, which results in a wrong computation

missing build instruction

theories/examples/delim_lang/example.v
@@ -9,27 +9,7 @@ Open Scope syn_scope.
 Example p : expr Empty_set :=
   ((#1) + (reset ((#3) + (shift/cc ((($0) @k #5) + (($0) @k #6)))))).
 
-Local Definition rs : gReifiers _ _ := gReifiers_cons reify_delim gReifiers_nil.
-(* Local Definition Hrs : subReifier reify_delim rs. *)
-(* Proof. unfold rs. apply subReifier_here. Qed. *)
-
-Notation F := (gReifiers_ops rs).
-Context {R} `{!Cofe R}.
-Context `{!SubOfe natO R, !SubOfe unitO R}.
-Notation IT := (IT F R).
-Notation ITV := (ITV F R).
-Context (env : @interp_scope F R _ Empty_set).
-
-Example ts := interp_config rs (Cexpr p) env.
-Definition t := fst ts.
-Definition σ := snd ts.
-
-
-Context `{!invGS Σ, !stateG rs R Σ, !heapG rs R Σ}.
-Notation iProp := (iProp Σ).
-
-
-Ltac shift_hom :=
+Global Ltac shift_hom :=
   match goal with
   | |- envs_entails _ (wp _ (ofe_mor_car _ _ (λne x, ?k1 x) (?k2 ?t)) _ _ _) =>
       assert ((ofe_mor_car _ _ (λne x, k1 x) (k2 t)) ≡ (λne x, k1 (k2 x)) t) as -> by done
@@ -37,74 +17,94 @@ Ltac shift_hom :=
       assert (k t ≡ (λne x, k x) t) as -> by done
   end.
 
-Ltac shift_natop_l :=
+Global Ltac shift_natop_l :=
   match goal with
   | |- envs_entails _ (wp _ (ofe_mor_car _ _ (λne x, ?k1 x)
-                               (ofe_mor_car _ _
-                                  (ofe_mor_car _ _
-                                     (NATOP (do_natop lang.Add)) ?t) (IT_of_V ?e))) _ _ _) =>
+                              (ofe_mor_car _ _
+                                 (ofe_mor_car _ _
+                                    (NATOP (do_natop lang.Add)) ?t) (IT_of_V ?e))) _ _ _) =>
       assert ((ofe_mor_car _ _ (λne x, k1 x) (NATOP (do_natop lang.Add) t (IT_of_V e))) ≡
                 (λne x, k1 (NATOP (do_natop lang.Add) x (IT_of_V e))) t) as -> by done
   end.
 
-Lemma wp_t (s : gitree.weakestpre.stuckness) :
-  has_substate σ -∗
-  WP@{rs} t @ s {{βv, βv ≡ RetV 18}}.
-Proof.
-  Opaque SHIFT APP_CONT.
-  iIntros "Hσ".
-  cbn.
-  (* first, reset *)
-  do 2 shift_hom.
-  iApply (wp_reset with "Hσ").
-  iIntros "!> _ Hσ". simpl.
+Section proof.
 
-  (* then, shift *)
-  do 2 shift_hom.
-  iApply (wp_shift with "Hσ").
-  { rewrite laterO_map_Next. done. }
-  iIntros "!>_ Hσ".
-  simpl.
+  Context {sz : nat}.
+  Variable rs : gReifiers CtxDep sz.
+  Context `{!subReifier reify_delim rs}.
 
-  (* the rest *)
-  rewrite -(IT_of_V_Ret 6) get_val_ITV'. simpl.
-  rewrite get_fun_fun. simpl.
-  do 2 shift_hom.
-  iApply (wp_app_cont with "Hσ"); first done.
-  iIntros "!> _ Hσ". simpl.
-  rewrite later_map_Next -Tick_eq.
-  iApply wp_tick. iNext.
-  shift_hom.
-  rewrite IT_of_V_Ret NATOP_Ret. simpl.
-  rewrite -(IT_of_V_Ret 9).
-  iApply (wp_pop_cons with "Hσ").
-  iIntros "!> _ Hσ".
-  simpl.
+  Notation F := (gReifiers_ops rs).
+  Context {R} `{!Cofe R}.
+  Context `{!SubOfe natO R}.
+  Notation IT := (IT F R).
+  Notation ITV := (ITV F R).
 
-  shift_hom. shift_natop_l.
-  rewrite -(IT_of_V_Ret 5) get_val_ITV'. simpl.
-  shift_hom. shift_natop_l.
-  rewrite get_fun_fun. simpl.
-  shift_hom. shift_natop_l.
-  iApply (wp_app_cont with "Hσ"); first done.
-  iIntros "!> _ Hσ". simpl.
-  rewrite later_map_Next -Tick_eq.
-  iApply wp_tick. iNext.
-  rewrite (IT_of_V_Ret 5) NATOP_Ret. simpl.
-  rewrite -(IT_of_V_Ret 8).
-  iApply (wp_pop_cons with "Hσ").
-  iIntros "!> _ Hσ".
-  simpl.
-  shift_hom.
-  shift_natop_l.
-  rewrite (IT_of_V_Ret 8).
-  simpl. rewrite IT_of_V_Ret NATOP_Ret.
-  simpl. rewrite -(IT_of_V_Ret 17).
-  iApply (wp_pop_cons with "Hσ").
-  iIntros "!> _ Hσ". simpl.
-  rewrite IT_of_V_Ret NATOP_Ret.
-  simpl. rewrite -(IT_of_V_Ret 18).
-  iApply (wp_pop_end with "Hσ").
-  iIntros "!> _ _".
-  iApply wp_val. done.
-Qed.
+  Context `{!invGS Σ, !stateG rs R Σ}.
+  Notation iProp := (iProp Σ).
+
+  Lemma wp_t σ (s : gitree.weakestpre.stuckness) :
+    (⊢ has_substate σ
+       -∗ WP@{rs} (interp_expr _ p ı_scope) @ s
+            {{ βv, βv ≡ RetV 18
+                   ∗ has_substate σ }})%I.
+  Proof.
+    Opaque SHIFT APP_CONT.
+    iIntros "Hσ".
+    cbn.
+    (* first, reset *)
+    do 2 shift_hom.
+    iApply (wp_reset with "Hσ").
+    iIntros "!> _ Hσ". simpl.
+
+    (* then, shift *)
+    do 2 shift_hom.
+    iApply (wp_shift with "Hσ").
+    { rewrite laterO_map_Next. done. }
+    iIntros "!>_ Hσ".
+    simpl.
+
+    (* the rest *)
+    rewrite -(IT_of_V_Ret 6) get_val_ITV'. simpl.
+    rewrite get_fun_fun. simpl.
+    do 2 shift_hom.
+    iApply (wp_app_cont with "Hσ"); first done.
+    iIntros "!> _ Hσ". simpl.
+    rewrite later_map_Next -Tick_eq.
+    iApply wp_tick. iNext.
+    shift_hom.
+    rewrite IT_of_V_Ret NATOP_Ret. simpl.
+    rewrite -(IT_of_V_Ret 9).
+    iApply (wp_pop_cons with "Hσ").
+    iIntros "!> _ Hσ".
+    simpl.
+
+    shift_hom. shift_natop_l.
+    rewrite -(IT_of_V_Ret 5) get_val_ITV'. simpl.
+    shift_hom. shift_natop_l.
+    rewrite get_fun_fun. simpl.
+    shift_hom. shift_natop_l.
+    iApply (wp_app_cont with "Hσ"); first done.
+    iIntros "!> _ Hσ". simpl.
+    rewrite later_map_Next -Tick_eq.
+    iApply wp_tick. iNext.
+    rewrite (IT_of_V_Ret 5) NATOP_Ret. simpl.
+    rewrite -(IT_of_V_Ret 8).
+    iApply (wp_pop_cons with "Hσ").
+    iIntros "!> _ Hσ".
+    simpl.
+    shift_hom.
+    shift_natop_l.
+    rewrite (IT_of_V_Ret 8).
+    simpl. rewrite IT_of_V_Ret NATOP_Ret.
+    simpl. rewrite -(IT_of_V_Ret 17).
+    iApply (wp_pop_cons with "Hσ").
+    iIntros "!> _ Hσ". simpl.
+    rewrite IT_of_V_Ret NATOP_Ret.
+    simpl. rewrite -(IT_of_V_Ret 18).
+    iApply wp_val.
+    iModIntro.
+    iFrame "Hσ".
+    done.
+  Qed.
+
+End proof.
